# Формулировка
$f:[a,b]\times[c,d]\to \mathbb{R}$
$f, f_t^\prime \in C([a, b]\times[c, d])$,   $\varphi, \psi : [c, d] \to [a, b]$ непр дифф
Тогда $F(t):=\int_{\varphi(t)}^{\psi(t)}f(x,t)d x \in C^1[c,d]$ и
$$F^\prime(t) = f(\psi(t), t)\psi^\prime(t) - f(\varphi(t), t)\varphi^\prime(t) + \int_{\varphi(t)}^{\psi(t)}f_t^\prime(x, t)dx$$
#MUSTHAVE 
# Доказательство
$\Phi(\alpha, \beta, t) = \int_\alpha^\beta f(x,t)d x \Rightarrow F(t) = \Phi(\varphi(t), \psi(t), t)$
$$F^\prime = \frac{\partial \Phi}{\partial\alpha}(\varphi(t), \psi(t), t)\varphi^\prime(t) + \frac{\partial \Phi}{\partial\beta}(\varphi(t), \psi(t), t)\psi^\prime(t) + \frac{\partial \Phi}{\partial t}(\varphi(t), \psi(t), t)$$
#TODO 
$$\frac{\partial\Phi}{\partial t}(\alpha, \beta, t) = \int_\alpha^\beta f_t^\prime(x, t)d$$
## Пример
$F(t) = \int_0^{+\infty}e^{-x^2}\cos(tx)dx$ 
$e^{-x^2}$ - суммируемая мажоранта $\Rightarrow f$ непрерывна на $\mathbb{R}$
$F^\prime(t)= \int_0^{+\infty}(e^{-x^2}\cos(tx))_t^\prime d x = -\int_0^{+\infty}\underbrace{e^{-x^2}x}{v^\prime}\underbrace{\sin(tx)dx}{u} =_*$
$xe^{-x^2}$ суммир мажоранта $\Rightarrow$ можно дифференциировать
$=_*  \frac{1}{2}e^{-x^2}\sin(tx)|_{x=0}^{x = +\infty} - \int_0^{+\infty}\frac{1}{2}e^{-x^2}t\cos(tx)dx = -\frac{t}{2}F(t)$
$F^\prime(t) + \frac{t}{2}F(t) = 0$
$\frac{F^\prime(t)}{F(t)}=-\frac{t}{2}\Rightarrow(\ln F(t))^\prime = -\frac{t}{2} \Rightarrow \ln F(t) = -\frac{t^2}{4} + C$, угадали что $F(t)e^{t^2/4} = const$
Проверим это $(F(t)e^{t^2/4})^\prime = F^\prime(t)e^{t^2/4} + F(t)e^{t^2/4}\frac{t}{2} = e^{t^2/4}(\underbrace{F^\prime(t) + \frac{t}{2}F(t)}{=0})=0$
Следовательно $F(t) = Ce^{-t^2/4}$ Найдём $C$, $C = F(0) = \int_0^{+\infty}e^{-x^2}dx = \frac{\sqrt{\pi}}{2}$
$F(t)=\frac{\sqrt{\pi}}{2}e^{-t^2/2}$
