# Формулировка 
$f \geq 0$ простая функция $A_1, \dots A_m\ и\ B_1, \dots, B_n$ её допустимые разбиения $a_1, \dots, a_m\ и\ b_1, \dots, b_n$ значения на соответствующих множествах
Тогда для любого измеримого множества $E$ ($X = \bscup\limits_{j=1}^{m}A_j = \bscup\limits_{k=1}^{n}B_k$)
$\sum\limits_{j=1}^{m}a_j \mu (E \bcap A_j) = \sum\limits_{k=1}^{n}b_k\mu(E\cap B_k)$
## Доказательство
Если $A_j \cap B_k \neq \varnothing$, то $a_j = b_k$
$\sum\limits_{j=1}^{m}a_j\mu(E\cap A_j) = \sum\limits_{j=1}^{m}\sum\limits_{k=1}^{n}a_j\mu(E\cap A_j \cap B_k)=$
$=\sum\limits_{j=1}^{m}\sum\limits_{k=1}^{n}b_k\mu(E\cap A_j \cap B_k) = \sum\limits_{k=1}^{n}b_k\mu(E\cap B_k)$
если $A_j \cap B_k = \varnothing$, то $\mu (E \cap A_j \cap B_k) = 0$
если $A_j \cap B_k \neq \varnothing$ то $a_j = b_k$
$\sum\limits_{j=1}^{m}\mu (E \cap A_j \cap B_k) = \mu (E \cap B_k)$
