# Теорема
$a$ - возвратная $\iff$ $\sum_{n=1}^\infty p_{aa}(n)$ расходится
Если $a$-невозвратное, то $F_a = \frac{P_a}{1 + P_a}$, где $P_a = \sum_{n=1}^\infty p_{aa}(n)$ 
## Доказательство
Положим $p_{aa}(0) = 1$ и $f_a(0) = 0$
$F(t) := \sum_{n=0}^\infty f_a(n) t^n$
$P(t) = \sum_{n=0}^\infty p_{aa}(n) t^n$ 
$p_{aa}(n) = f_a(n) + f_a(n-1) p_{aa}(1) + ... = \sum_{k=0}^n f_a(k) p_{aa} (n - k)$ при $n > 0$
$P(T) F(T) = P(T) + 1$ 
$F(t) = 1 - \frac{1}{P(T)}$
$$\lim F(t)_{t \to 1-} F(t) = 1 - \lim_{t \to 1-} \frac{1}{P(t)}$$
Если $1 + P_a = \sum_{n=0}^\infty < +\infty$, то $\lim_{t \to 1-} P(t) = P_a + 1$ 
При бесконечности это бесконечность
# Следствие
Невозвратное состояние обязательно нулевое
## Доказательство
Члены ряда стремятся с нулю