# Теорема
$f \in H(\Omega), a \in \Omega, \overline{B}_r(a) \in \Omega$
$$f(a) = \frac{1}{2\pi} \int_{0}^{2\pi} f(a + re^{it})dt$$
## Доказательство
$$f(a) = \frac{1}{2\pi i} \int_{|z - a| = r} \frac{f(z)}{z -a} dz = \frac{1}{2\pi i} \int_{0}^{2\pi} f(a + re^{it}) \frac{r \cdot i \cdot e^{it}}{e \cdot e^{it}}dt $$$$= \frac{1}{2\pi} \int_{0}^{2\pi} f(a + re^{it}) dt$$

Параметризация $\gamma(t) = a + re^{it}$ 

$\gamma^\prime(t) = ire^{it}$
# Следствие
$f \in H(\Omega), a \in \Omega$. $\overline{B}_r(a) \sub \Omega$. Тогда $$f(a) = \frac{1}{\pi r^2} \int_{|z - a| \leq r} f(z) d \lambda_2$$
## Доказательство
$$\int_{|z - a| \leq r} f(z) d\lambda_2 = \int_{0}^r \int_{0}^{2\pi} f(a + \rho e^{it})\rho \ dt \ d\rho = \int_0^r\rho \int_{0}^{2\pi}f(a + \rho e^{it}) dt d\rho$$
$$=\int_0^r\rho  d\rho \cdot 2\pi f(a) = r^2\pi f(a)$$